feat: `UnTyped` projections and docstrings. Rename `Program` to `Body`

LeanMlirCommon/UnTyped/Basic.lean
@@ -1,16 +1,10 @@
 
 namespace MLIR
 
---TODO: fix this doc now that `Var` is gone
-/-- `VarName` is the type of (human-readable) variable names.
-Variables names are primarily used at when binding new variables, whereas the `Var` generic type
-is used
-
-The name _might_ be semantically significant (in particular, when `Var = VarName`), or it might
-be used only for pretty printing (for example, when we use De-Bruijn indices for `Var`). -/
+/-- `VarName` is the type of (human-readable) variable names -/
 def VarName : Type := String
 
-/-- `BlockLabel` is the type of (human-readable) basic block labels. -/
+/-- `BlockLabel` is the type of (human-readable) basic block labels -/
 def BlockLabel : Type := String
 
 instance : DecidableEq VarName := by unfold VarName; infer_instance
@@ -29,19 +23,20 @@ mutual
 inductive Expr
   | mk (varName : VarName) (op : Op) (args : List VarName) (regions : List Region)
 
-/-- `Lets` is a sequence of operations (without terminator) -/
+/-- `Lets` is a sequence of operations (without terminator), which grows downwards.
+That is, the head of the list represents the first operation to be executed -/
 inductive Lets
   | mk (lets : List Expr)
 
-/-- `Program` is a sequence of operations, followed by a terminator -/
-inductive Program
+/-- The `Body` of a basic block is a sequence of operations, followed by a terminator -/
+inductive Body
   | mk (lets : Lets) (terminator : T)
 
 /-- A basic block has a label, a set of arguments, and then a program -/
 inductive BasicBlock
-  | mk (label : BlockLabel) (args : List VarName) (program : Program)
+  | mk (label : BlockLabel) (args : List VarName) (body : Body)
 
-/-- A regions consists of one or more basic blocks, where the first basic block is known as the
+/-- A region consists of one or more basic blocks, where the first basic block is known as the
 entry block -/
 inductive Region
   | mk (entry : BasicBlock) (blocks : List BasicBlock)
@@ -50,9 +45,30 @@ end
 
 
 /-! ## Projections -/
-namespace Expr
+variable {Op T : Type}
 
-def varName : Expr Op T → VarName
+def Expr.varName : Expr Op T → VarName
   | ⟨varName, _, _, _⟩ => varName
+def Expr.op : Expr Op T → Op
+  | ⟨_, op, _, _⟩ => op
 
-end Expr
+@[simp] theorem Expr.op_mk {varName} {op : Op} {args} {regions : List (Region Op T)} :
+    Expr.op ⟨varName, op, args, regions⟩ = op := rfl
+@[simp] theorem Expr.varName_mk {varName} {op : Op} {args} {regions : List (Region Op T)} :
+    Expr.varName ⟨varName, op, args, regions⟩ = varName := rfl
+
+def Lets.inner : Lets Op T → List (Expr Op T)
+  | ⟨inner⟩ => inner
+
+@[simp] theorem Lets.mk_inner (lets : Lets Op T) : ⟨lets.inner⟩ = lets := by cases lets; rfl
+@[simp] theorem Lets.inner_mk (lets : List (Expr Op T)) : Lets.inner ⟨lets⟩ = lets := rfl
+
+namespace BasicBlock
+
+def args : BasicBlock Op T → List VarName
+  | ⟨_, args, _⟩ => args
+
+def body : BasicBlock Op T → Body Op T
+  | ⟨_, _, body⟩ => body
+
+end BasicBlock
